src/ListBackInd.v
@@ -7,43 +7,15 @@ Import ListNotations.
 Require Import PathToSubtree.
 Require Import HLPL.
 
-
-Theorem list_back_ind : forall (A : Type) (P : list A -> Prop) (Hnil : P []) (Hrec : (forall (a : A) (l : list A), P l -> P (l ++ [a]))), forall (l : list A), P l.
-Proof.
-  intros A P Hnil Hrec l. 
-  remember (length l) as len. generalize dependent l.
-  induction len ; intros l Heqlen.
-  - symmetry in Heqlen. apply length_zero_iff_nil in Heqlen. subst ; auto.
-  - destruct l ; simpl in Heqlen.
-    * discriminate.
-    * injection Heqlen as Heqlen.
-      remember (rev (a :: l)) as alrev.
-      destruct alrev as [ | b l'].
-    + apply f_equal with (f := @length A) in Heqalrev.
-      simpl in Heqalrev. rewrite length_app, Nat.add_comm in Heqalrev.
-      simpl in Heqalrev. congruence.
-    + specialize (Hrec b (rev l')).
-      assert (H : len = length (rev l')).
-      {
-        apply f_equal with (f := @length A) in Heqalrev.
-        simpl in Heqalrev. rewrite length_app, Nat.add_comm in Heqalrev.
-        simpl in Heqalrev. injection Heqalrev ; intros ; auto.
-        rewrite length_rev. rewrite length_rev in H. congruence.
-      }
-      specialize (IHlen (rev l') H). specialize (Hrec IHlen).
-      assert (H' : rev (b :: l') = rev (rev (a :: l))) by congruence.
-      rewrite rev_involutive in H'. rewrite <- H'. simpl. auto.
-Qed.
-
 Theorem state_path_back_ind : forall (P : spath -> Prop) (Hbase : forall enc_x, P (enc_x, [])) (Hrec : (forall (n : nat) (sp : spath), P sp -> P (sp +++ [n]))), forall (sp : spath), P sp.
 Proof.
   intros P Hbase Hrec sp. rewrite surjective_pairing with (p := sp).
   remember (snd sp) as vp. generalize dependent sp.
-  induction vp using list_back_ind ; intros sp Hsnd.
+  induction vp using rev_ind ; intros sp Hsnd.
   - apply Hbase.
   - remember (fst sp, vp) as sp'.
     rewrite Hsnd, <- surjective_pairing.
-    replace sp with (sp' +++ [a]).
+    replace sp with (sp' +++ [x]).
     * apply Hrec. rewrite surjective_pairing with (p := sp') in Heqsp'.
       apply base.pair_eq in Heqsp'. destruct Heqsp' as [H1 H2].
       rewrite surjective_pairing. rewrite <- H2 in IHvp.
